Try making IOEffects an applicative functor

Shenzhen/IOEffects.lean
@@ -5,87 +5,138 @@ import Shenzhen.SimpleIOData
   We also record reads and writes from simple I/O pins, although they don't block.
   - `ξ` is the type of *X*Bus pins.
   - `ι` is the type of simple *I*/O pins.-/
-inductive IOEffects (ξ : Type u) (ι : Type v) (α : Type x)
+inductive IOEffects (ξ : Type u) (ι : Type v) : Type x → Type (max u v _)
 /-- Just return a value immediately, without doing any effects. -/
-| pure (a : α)
+| pure (a : α) : IOEffects _ _ α
 /-- `xBusRead pin next` represents a computation delayed until a value `d`
   from `pin` can be read; then `next d` is the result of the computation. -/
-| xBusRead (pin : ξ) (next : Integer → IOEffects ξ ι α)
+| xBusRead (pin : ξ) (next : IOEffects ξ ι (Integer → α)) : IOEffects _ _ α
 /-- `d` is some data to be thereafter written out of `outPin`, and `next ()` is returned after the write. -/
-| xBusWrite (outPin : ξ) (d : Integer) (next : Unit → IOEffects ξ ι α)
+| xBusWrite (outPin : ξ) (d : Integer) (next : IOEffects ξ ι α) : IOEffects _ _ α
 /-- `xBusPoll pin next` represents a computation delayed until the value
   from XBus pin `pin` arrives (but without consuming the value);
   then `next ()` is the result thereafter.
   This is used to implement the `slx` instruction. -/
-| xBusPoll (pin : ξ) (next : Unit → IOEffects ξ ι α)
-| simpleIORead (pin : ι) (next : SimpleIOData → IOEffects ξ ι α)
-| simpleIOWrite (outPin : ι) (d : SimpleIOData) (next : Unit → IOEffects ξ ι α)
+| xBusPoll (pin : ξ) (next : IOEffects ξ ι α) : IOEffects _ _ α
+| simpleIORead (pin : ι) (next : IOEffects ξ ι (SimpleIOData → α)) : IOEffects _ _ α
+| simpleIOWrite (outPin : ι) (d : SimpleIOData) (next : IOEffects ξ ι α) : IOEffects _ _ α
 /-- Wait for `n` time units. -/
-| sleep (n : Nat) (h : n ≠ 0) (next : Unit → IOEffects ξ ι α)
+| sleep (n : Nat) (h : n ≠ 0) (next : IOEffects ξ ι α) : IOEffects _ _ α
 
 namespace IOEffects
 
 instance [Inhabited α] : Inhabited (IOEffects ξ ι α) :=
   ⟨pure default⟩
 
-
+@[simp]
 instance : Pure (IOEffects ξ ι) where
   pure := .pure
 
 @[simp]
-def bind (mx : IOEffects ξ ι α) (f : α → IOEffects ξ ι β) : IOEffects ξ ι β :=
-  match mx with
-  | pure a => f a
-  | .xBusRead p next => .xBusRead p fun d => bind (next d) f
-  | .simpleIORead p next => .simpleIORead p fun d => bind (next d) f
-  | .xBusWrite p d next => .xBusWrite p d fun () => bind (next ()) f
-  | .simpleIOWrite p d next => .simpleIOWrite p d fun () => bind (next ()) f
-  | xBusPoll p next => xBusPoll p fun () => bind (next ()) f
-  | .sleep n h next => .sleep n h fun () => bind (next ()) f
+def map (f : α → β) : IOEffects ξ ι α → IOEffects ξ ι β
+  | .pure a => .pure (f a)
+  | .xBusRead pin next => .xBusRead pin (map (f ∘ ·) next)
+  | .xBusWrite pin d next => .xBusWrite pin d (map f next)
+  | .xBusPoll pin next => .xBusPoll pin (map f next)
+  | .simpleIORead pin next => .simpleIORead pin (map (f ∘ ·) next)
+  | .simpleIOWrite pin d next => .simpleIOWrite pin d (map f next)
+  | .sleep n h next => .sleep n h (map f next)
 
-instance : Monad (IOEffects ξ ι) where
-  bind := bind
+instance : Functor (IOEffects ξ ι) where
+  map := map
+
+@[simp, reducible]
+def _root_.Function.swap {α β γ} (f : α → β → γ) : β → α → γ :=
+  fun b a => f a b
+
+@[simp] -- simp needed for decreasing proof in `seq` and decreasing proofs for lawful applicative theorems below
+theorem sizeOf_map_eq_sizeOf {f : α → β} {fx : IOEffects ξ ι α} : sizeOf (map f fx) = sizeOf fx := by
+  induction fx generalizing β <;> simp_all [map]
+
+@[simp]
+def seq (mf : IOEffects ξ ι (α → β)) (mx : Unit → IOEffects ξ ι α) : IOEffects ξ ι β :=
+  match mf with
+  | .pure f => f <$> mx ()
+  | .xBusRead pin nextF => .xBusRead pin (seq (map Function.swap nextF) mx)
+  | .xBusWrite pin d nextF => .xBusWrite pin d (seq nextF mx)
+  | .xBusPoll pin nextF => .xBusPoll pin (seq nextF mx)
+  | .simpleIORead pin nextF => .simpleIORead pin (seq (map Function.swap nextF) mx)
+  | .simpleIOWrite pin d nextF => .simpleIOWrite pin d (seq nextF mx)
+  | .sleep n h nextF => .sleep n h (seq nextF mx)
+termination_by sizeOf mf
+decreasing_by all_goals simp [sizeOf_map_eq_sizeOf, show ∀ n, 0 < 1 + n by omega]
+
+instance : Applicative (IOEffects ξ ι) where
+  seq := seq
 
 section
 
 -- TODO: make this local
 attribute [simp] Functor.map Seq.seq Bind.bind Pure.pure
 
-theorem id_map (x : IOEffects ξ ι α) : id <$> x = x := by
-  induction x <;> try rfl
-  all_goals
-    simp; rename_i ih; funext; apply ih
-
-theorem bind_pure_comp (f : α → β) (x : IOEffects ξ ι α) : x >>= (fun a => pure (f a)) = f <$> x := by
+private theorem id_map (x : IOEffects ξ ι α) : id <$> x = x := by
   induction x
-  all_goals
-    simp <;> rename_i ih <;> funext <;> apply ih
+  all_goals first | rfl | simp; rename_i ih; funext; apply ih
 
-instance : LawfulMonad (IOEffects ξ ι) where
+theorem _root_.Function.comp_assoc {f : γ → δ} {g : β → γ} {h : α → β} : (f ∘ g) ∘ h = f ∘ (g ∘ h) :=
+  rfl
+
+private theorem comp_map (g : α → β) (h : β → γ) (x : IOEffects ξ ι α) : (h ∘ g) <$> x = h <$> g <$> x := by
+  induction x generalizing β γ
+  <;> simp_all
+  <;> (rename_i ih; exact ih (h := fun x => h ∘ x) (g := fun x => g ∘ x))
+
+private theorem comp_map' {α β γ : Type u} {x : IOEffects ξ ι α} {f : β → γ} {g : α → β} : map f (map g x) = map (f ∘ g) x :=
+  (comp_map ..).symm
+
+private theorem seq_pure (g : IOEffects ξ ι (α → β)) (x : α)
+    : g.seq (fun _ => pure x) = g.map (fun h => h x) := by
+  cases g
+  all_goals first
+    | (simp; done)
+    | (unfold seq; congr; apply seq_pure)
+    | (unfold seq; congr; rw [seq_pure, comp_map']; rfl)
+
+private theorem seq_map_r {f : α → β} {mh : IOEffects ξ ι (β → γ)} {x : IOEffects ξ ι α}
+    : (mh.seq fun () => map f x) = (map (· ∘ f) mh).seq fun () => x := by
+  cases mh <;> first
+    | simp [comp_map']; done
+    | simp only [seq, map, comp_map', xBusRead.injEq, true_and]; rw [seq_map_r, comp_map']; rfl
+    | simp only [seq, map, xBusWrite.injEq, true_and]; rw [seq_map_r]
+
+private theorem seq_map_l {α β γ : Type u} {f : α → β} {mx : IOEffects ξ ι α} {mg : IOEffects ξ ι (β → γ)}
+    : ((map (· ∘ f) mg).seq fun () => mx) = ((map Function.comp mg).seq fun _ => pure f).seq fun () => mx := by
+  cases mg
+  all_goals congr 3; simp only [comp_map', seq_pure]; rfl
+
+private theorem map_seq_r {f : β → γ} {mg : IOEffects ξ ι (α → β)} {x : IOEffects ξ ι α}
+    : map f (mg.seq fun () => x) = (map (Function.comp f) mg).seq fun () => x := by
+  cases mg <;> first
+    | simp [comp_map']; done
+    | simp only [seq, map]; rw [map_seq_r]; simp only [comp_map']; rfl
+    | simp only [seq, map]; rw [map_seq_r]
+
+private theorem seq_assoc (x : IOEffects ξ ι α) (g : IOEffects ξ ι (α → β)) (h : IOEffects ξ ι (β → γ))
+    : h.seq (fun _ => g.seq fun _ => x) = ((h.map Function.comp).seq fun _ => g).seq fun _ => x := by
+  cases h <;> first
+    | simp [map_seq_r]; done
+    | simp only [seq, map, comp_map']; rw [seq_assoc]; simp only [comp_map', map_seq_r]; rfl
+    | simp only [seq, map]; rw [seq_assoc]
+
+instance : LawfulApplicative (IOEffects ξ ι) where
   map_const := rfl
   id_map := id_map
-  seqLeft_eq x y := by
-    simp [SeqLeft.seqLeft]
-    induction x
-    all_goals
-      first | apply bind_pure_comp | rename_i ih; funext; simp [ih]
-  seqRight_eq x y := by
-    simp [SeqRight.seqRight]
-    induction x
-    all_goals
-      first | symm; apply id_map | rename_i ih; funext; simp [ih]
-  pure_seq f x := by simp [Seq.seq]
-  bind_pure_comp := bind_pure_comp
-  bind_map f x := by
-    induction f <;> simp <;> (rename_i ih; funext; apply ih)
-  pure_bind := by simp
-  bind_assoc x f g := by
-    induction x <;> simp <;> (rename_i ih; funext; apply ih)
+  seqLeft_eq x y := rfl
+  seqRight_eq x y := rfl
+  pure_seq f x := by simp
+  map_pure := by simp
+  seq_pure := seq_pure
+  seq_assoc := seq_assoc
 
 end
 
 def sleepOne : IOEffects ξ ι α → IOEffects ξ ι α
-| .sleep 1 _ next => next ()
+| .sleep 1 _ next => next
 | .sleep (k + 2) _ next => .sleep (k + 1) (Nat.succ_ne_zero _) next
 | fx => fx
 
